proof/invariant-abstract/ARM/ArchDetSchedSchedule_AI.thy
@@ -162,9 +162,9 @@ lemma switch_to_idle_thread_ct_not_queued [wp, DetSchedSchedule_AI_assms]:
                          pred_tcb_at_def obj_at_def not_queued_def)
   done
 
-crunch valid_blocked_except_set[wp]: set_vm_root "\<lambda>s.
-           valid_blocked_except_set_2 {} (ready_queues s) (release_queue s) (kheap s)
-            (scheduler_action s) thread"
+crunch valid_blocked_except_set[wp]: set_vm_root
+  "\<lambda>s. valid_blocked_except_set_2 {} (ready_queues s) (release_queue s) (kheap s)
+       (scheduler_action s) thread"
   (wp: crunch_wps simp: crunch_simps)
 
 lemma switch_to_idle_thread_valid_blocked [wp, DetSchedSchedule_AI_assms]:
